polydecidable eq const

src/polycodable.lean
@@ -4,10 +4,8 @@ import pfun_to_fun
 import polytime
 
 
-structure polydecidable_aux (P : ptree → Prop) :=
-(c : code)
-(pc : polytime c)
-(sound : ∀ x, ptree.nil ∈ c.eval x ↔ P x)
+def polydecidable_aux (P : ptree → Prop) : Prop :=
+∃ (c : code) (pc : polytime c), ∀ x, ptree.nil ∈ c.eval x ↔ P x 
 
 -- lemma polydecidable_code_eval_nil_iff (P : ptree → Prop) [h : polydecidable P] (x : ptree) :
 --   (h.c.eval.to_fun h.pc.dom_univ x = ptree.nil) ↔ P x :=
@@ -72,49 +70,100 @@ structure polydecidable_aux (P : ptree → Prop) :=
 
 class polycodable (α : Type*) :=
 (encode : α ↪ ptree)
-(mem_poly : polydecidable_aux (∈ set.range encode))
+(mem_poly' : polydecidable_aux (∈ set.range encode))
 
--- class polydecidable {α : Type*} (P : α → Prop) : 
-
-open polycodable
+open polycodable (encode)
 
 instance : polycodable ptree :=
-⟨function.embedding.refl _, by { simp, apply_instance, }⟩
+{ encode := function.embedding.refl _,
+  mem_poly' := ⟨code.nil, polytime_nil, by simp⟩ }
 
-@[simp] lemma range_of_surjective_comp {α β γ : Type*} (f : α → β) (g : β → γ) (hf : function.surjective f) :
-  set.range (g ∘ f) = set.range g :=
-begin
-  ext y, split, { rintro ⟨x, hx⟩, use f x, exact hx, },
-  rintro ⟨x', rfl⟩,
-  obtain ⟨x, rfl⟩ := hf x',
-  use x,
-end
+@[simp] lemma ptree_encode (p : ptree) : encode p = p := rfl
 
+variables {α β γ : Type*} [polycodable α] [polycodable β] [polycodable γ]
 
-def polycodable_of_equiv {α β : Type*} [polycodable α] (h : α ≃ β) : polycodable β :=
-⟨h.symm.to_embedding.trans encode, 
-begin
-  simp only [function.embedding.trans, function.embedding.coe_fn_mk, function.comp_app, equiv.to_embedding_apply],
-  rw range_of_surjective_comp, { apply_instance, }, { exact h.symm.surjective, },
-end⟩
+def polydecidable (P : α → Prop) : Prop :=
+∃ (c : code) (pc : polytime c), ∀ x, ptree.nil ∈ c.eval (encode x) ↔ P x   
 
-structure polytime_fun {α β : Type*} [polycodable α] [polycodable β] (f : α → β) :=
-(c : code)
-(pc : polytime c)
-(sound : ∀ x : α, c.eval (encode x) = part.some (encode (f x)))
+@[simp] lemma polydecidable_aux_iff (P : ptree → Prop) : polydecidable_aux P ↔ polydecidable P :=
+⟨λ ⟨c, pc, sound⟩, ⟨c, pc, sound⟩, λ ⟨c, pc, sound⟩, ⟨c, pc, sound⟩⟩
+
+def polytime_fun {α β : Type*} [polycodable α] [polycodable β] (f : α → β) :=
+∃ (c : code) (pc : polytime c), ∀ x, c.eval (encode x) = part.some (encode (f x))
 
 section polytime_fun
-variables {α β : Type*} [polycodable α] [polycodable β]
 
--- lemma polydecidable_of_preimage_polytime {f : β → α} (hf : polytime_fun f) (P : α → Prop) [h : polydecidable P]
+lemma polydecidable_of_preimage_polytime {f : β → α} {P : α → Prop}  :
+  polytime_fun f → polydecidable P → polydecidable (λ y, P (f y))
+| ⟨c₁, pc₁, sound₁⟩ ⟨c₂, pc₂, sound₂⟩ := ⟨c₂.comp c₁, polytime_comp pc₂ pc₁, λ y, by simp [sound₁, sound₂]⟩
+
+lemma polytime_fun.id : polytime_fun (@id α) := ⟨code.id, polytime_id, λ x, by simp⟩
+
+lemma polytime_fun.const (x : α) : polytime_fun (function.const β x) := ⟨code.const (encode x), polytime_const _, λ x, by simp⟩
+
+lemma polytime_fun.comp {f : β → γ} {g : α → β} : polytime_fun f → polytime_fun g → polytime_fun (f ∘ g)
+| ⟨c₁, pc₁, s₁⟩ ⟨c₂, pc₂, s₂⟩ := ⟨c₁.comp c₂, polytime_comp pc₁ pc₂, λ x, by simp [s₁, s₂]⟩
+
+lemma polytime_fun.ptree_left : polytime_fun ptree.left := ⟨code.left, polytime_left, λ x, by simp⟩
+lemma polytime_fun.ptree_right : polytime_fun ptree.right := ⟨code.right, polytime_right, λ x, by simp⟩
+
+protected lemma polytime_fun.ite {c : α → Prop} [decidable_pred c] {t : α → β} {f : α → β} :
+  polydecidable c → polytime_fun t → polytime_fun f → polytime_fun (λ x, if c x then t x else f x)
+| ⟨c₁, pc₁, s₁⟩ ⟨c₂, pc₂, s₂⟩ ⟨c₃, pc₃, s₃⟩ :=
+⟨code.ite c₁ c₂ c₃, polytime_ite pc₁ pc₂ pc₃, λ x, 
+begin
+  specialize s₁ x, specialize s₂ x, specialize s₃ x,
+  by_cases h : c x,
+  { simp only [h, iff_true, ← part.eq_some_iff] at s₁, simp [h, s₁, s₂], },
+  { simp only [h, iff_false] at s₁,
+    obtain ⟨v, hv⟩ := (_ : ∃ v, v ∈ c₁.eval (encode x)),
+    have : v ≠ ptree.nil := by { rintro rfl, contradiction, },
+    { rw ← part.eq_some_iff at hv, simp [h, hv, this, s₃], },
+    rw ← part.dom_iff_mem, exact pc₁.dom_univ' _, }
+end⟩
+
+lemma polydecidable.or {P₁ P₂ : α → Prop} : polydecidable P₁ → polydecidable P₂ → polydecidable (λ x, (P₁ x) ∨ (P₂ x)) :=
+begin
+  classical,
+  rintros h₁ ⟨c₂, pc₂, s₂⟩,
+  suffices : polytime_fun (λ x, if P₁ x then ptree.nil else c₂.eval.to_fun pc₂.dom_univ (encode x)),
+  { rcases this with ⟨c, pc, s⟩, use [c, pc], intro x,
+    by_cases h : P₁ x, { simp [s, h], },
+    simp [s, h, pfun.to_fun, s₂], },
+  apply polytime_fun.ite h₁ (polytime_fun.const _) ⟨c₂, pc₂, _⟩,
+  intro x, simp [pfun.to_fun],
+end
+
+lemma polydecidable.not {P : α → Prop} (h : polydecidable P) : polydecidable (λ x, ¬P x) :=
+begin
+  classical,
+  suffices : polytime_fun (λ x, if P x then ptree.node ptree.nil ptree.nil else ptree.nil),
+  { rcases this with ⟨c, pc, s⟩, use [c, pc], intro x, simp [s x], split_ifs; simpa, },
+  apply polytime_fun.ite h (polytime_fun.const _) (polytime_fun.const _),
+end
+
+lemma polydecidable.and {P₁ P₂ : α → Prop} (h₁ : polydecidable P₁) (h₂ : polydecidable P₂) : polydecidable (λ x, (P₁ x) ∧ (P₂ x)) :=
+begin
+  simp only [and_iff_not_or_not],
+  apply polydecidable.not, apply polydecidable.or; apply polydecidable.not; assumption,
+end
+
+private lemma eq_nil_aux : polydecidable (=ptree.nil) := ⟨code.id, polytime_id, λ x, by { simp, exact comm, }⟩
+private lemma eq_const_aux : ∀ (x : ptree), polydecidable (=x)
+| ptree.nil := eq_nil_aux
+| (ptree.node a b) :=
+begin
+  convert_to polydecidable (λ x, x ≠ ptree.nil ∧ x.left = a ∧ x.right = b),
+  { ext x, cases x; simp, },
+  apply polydecidable.and, apply polydecidable.not eq_nil_aux, apply polydecidable.and,
+  exact polydecidable_of_preimage_polytime polytime_fun.ptree_left (eq_const_aux a),
+  exact polydecidable_of_preimage_polytime polytime_fun.ptree_right (eq_const_aux b),
+end
+
+lemma polydecidable.eq_const (x : α) : polydecidable (=x) :=
+let ⟨c, pc, s⟩ := eq_const_aux (encode x) in ⟨c, pc, λ x', by simpa using s (encode x')⟩
+
+
 
 end polytime_fun
 
-instance (α β : Type*) [polycodable α] [polycodable β] : polycodable (α × β) :=
-⟨⟨λ x, ptree.node (encode x.1) (encode x.2), λ x y, by { simp only [prod.ext_iff, embedding_like.apply_eq_iff_eq, and_imp], exact and.intro, }⟩, 
-begin
-  convert_to polydecidable (λ x, ¬(x = ptree.nil)), swap,
-  { haveI := polydecidable_eq_nil, apply_instance, },
-  ext x, simp only [set.mem_range, function.embedding.coe_fn_mk, prod.exists], split, { rintro ⟨a, b, rfl⟩, simp, },
-  cases x with a b, { intro, contradiction, }, intro _,
-end⟩
